\documentclass[12pt]{article}

\usepackage{amsmath, amssymb}
\usepackage{geometry}
\usepackage{setspace}
\usepackage{titlesec}
\usepackage{lmodern}
\usepackage{xcolor}
\usepackage{enumitem}

\geometry{margin=1in}
\setstretch{1.2}
\titleformat{\section}{\normalfont\Large\bfseries}{\thesection}{1em}{}
\titleformat{\subsection}{\normalfont\large\bfseries}{\thesubsection}{1em}{}
\pagenumbering{gobble}

\begin{document}

\begin{center}
    \LARGE \textbf{Unit 6: Quadratic and Polynomial Functions} \\[6pt]
    \Large \textbf{Topic 5: Adding, Subtracting, and Multiplying Polynomials}
\end{center}

\vspace{1em}

\section*{Concept Summary}

Polynomials are algebraic expressions made up of terms that include variables raised to whole-number powers.  
Examples: \(3x^2 + 5x - 2\), \(x^3 - 4x\), and \(2x^2 + 7\).

Operations on polynomials follow the same rules as arithmetic, except that we combine \textbf{like terms}—those with the same variable and exponent.

\[
\text{Like terms: } 4x^2 \text{ and } -3x^2 \quad \text{(both have } x^2\text{)}
\]
\[
\text{Unlike terms: } x^2 \text{ and } x^3
\]

\subsection*{1. Adding and Subtracting Polynomials}
To add or subtract, align like terms and combine their coefficients.

\[
(3x^2 + 2x + 5) + (4x^2 - x - 2) = 7x^2 + x + 3
\]
\[
(5x^3 - 2x^2 + x) - (3x^3 + 4x - 6) = 2x^3 - 2x^2 - 3x + 6
\]

\subsection*{2. Multiplying Polynomials}
Use the \textbf{Distributive Property} or \textbf{FOIL} for binomials:
\[
(a + b)(c + d) = ac + ad + bc + bd
\]

\[
(x + 3)(x + 5) = x^2 + 8x + 15
\]

When multiplying larger polynomials, multiply each term in one by each term in the other and then combine like terms.

\[
(x + 2)(x^2 + 3x + 4) = x^3 + 3x^2 + 4x + 2x^2 + 6x + 8 = x^3 + 5x^2 + 10x + 8
\]

\subsection*{3. Special Products to Remember}
\[
(a + b)^2 = a^2 + 2ab + b^2
\]
\[
(a - b)^2 = a^2 - 2ab + b^2
\]
\[
(a + b)(a - b) = a^2 - b^2
\]

Recognizing these patterns can save time on the SAT.

\section*{Core Skills}
\begin{itemize}
  \item Identify and combine like terms correctly.
  \item Apply distributive property to multiply expressions.
  \item Recognize and expand special product patterns.
  \item Simplify expressions by collecting terms and ordering by degree.
  \item Apply these operations in context problems (area, expansion, algebraic structure).
\end{itemize}

\section*{Example 1: Adding Polynomials}

Simplify:
\[
(2x^2 + 3x - 4) + (x^2 - 5x + 6)
\]

Combine like terms:
\[
(2x^2 + x^2) + (3x - 5x) + (-4 + 6) = 3x^2 - 2x + 2.
\]

\textbf{Result:} \(\boxed{3x^2 - 2x + 2}\)

\section*{Example 2: Subtracting Polynomials}

Simplify:
\[
(4x^3 - 2x + 5) - (x^3 + 3x - 7)
\]

Distribute the negative:
\[
4x^3 - 2x + 5 - x^3 - 3x + 7 = 3x^3 - 5x + 12.
\]

\textbf{Result:} \(\boxed{3x^3 - 5x + 12}\)

\section*{Example 3: Multiplying Binomials (FOIL)}

Simplify:
\[
(x + 4)(x + 6)
\]

Use FOIL (First, Outer, Inner, Last):
\[
x^2 + 6x + 4x + 24 = x^2 + 10x + 24.
\]

\textbf{Result:} \(\boxed{x^2 + 10x + 24}\)

\section*{Example 4: Difference of Squares}

Simplify:
\[
(3x + 5)(3x - 5)
\]
\[
= (3x)^2 - 5^2 = 9x^2 - 25.
\]

\textbf{Result:} \(\boxed{9x^2 - 25}\)

\section*{Example 5: Squaring a Binomial}

Simplify:
\[
(x + 3)^2 = (x + 3)(x + 3) = x^2 + 6x + 9.
\]

\textbf{Result:} \(\boxed{x^2 + 6x + 9}\)

\section*{Example 6: Area Application}

The length of a rectangle is \((x + 4)\) and the width is \((x + 2)\).  
Find the area as a polynomial.

\[
A = (x + 4)(x + 2) = x^2 + 6x + 8.
\]

\textbf{Area:} \(\boxed{x^2 + 6x + 8}\)

\section*{Key Takeaways}
\begin{itemize}
  \item Combine only like terms when adding or subtracting.
  \item Apply distributive property for multiplication.
  \item Recognize shortcuts for special products to save time.
  \item Always simplify and arrange terms in descending powers.
  \item These operations appear in both algebraic and geometric SAT contexts.
\end{itemize}

\newpage

% ============================================================
% QUESTIONS — UNIT 6, TOPIC 5: ADDING, SUBTRACTING, AND MULTIPLYING POLYNOMIALS
% ============================================================

\section*{Practice Questions: Adding, Subtracting, and Multiplying Polynomials}

\subsection*{Part A: Adding and Subtracting Simple Polynomials}
\begin{enumerate}
  \item Simplify: \((3x^2 + 5x + 2) + (4x^2 + 3x - 7)\)
  \item Simplify: \((6x^2 - 2x + 9) - (x^2 + 4x - 3)\)
  \item Simplify: \((5x^3 - 2x + 1) + (3x^3 + x - 4)\)
  \item Simplify: \((2x^4 + 7x^2 - 3) - (x^4 - 2x^2 + 6)\)
  \item Simplify: \((4x^3 + 2x^2 - 5x) - (6x^3 - 3x^2 + x)\)
\end{enumerate}

\subsection*{Part B: Combining Like Terms and Simplifying Expressions}
\begin{enumerate}
  \setcounter{enumi}{5}
  \item Simplify: \(3x^2 + 2x - 5 + 7x^2 - 4x + 9\)
  \item Simplify: \(2x^3 - 4x + 6 - (x^3 + 5x - 2)\)
  \item Simplify: \(5x^4 + 3x^2 - (2x^4 - 7x^2 + 8)\)
  \item Simplify: \((x^2 + 4x + 1) + (2x^2 - 6x + 9)\)
  \item Simplify: \((x^3 - 5x + 3) - (2x^3 - 4x + 8)\)
\end{enumerate}

\subsection*{Part C: Multiplying Binomials (FOIL Method)}
\begin{enumerate}
  \setcounter{enumi}{10}
  \item Expand: \((x + 3)(x + 7)\)
  \item Expand: \((x - 2)(x + 5)\)
  \item Expand: \((2x + 4)(x + 1)\)
  \item Expand: \((3x - 2)(x - 5)\)
  \item Expand: \((x + 6)^2\)
\end{enumerate}

\subsection*{Part D: Recognizing Special Products}
\begin{enumerate}
  \setcounter{enumi}{15}
  \item Expand: \((a + b)^2\)
  \item Expand: \((a - b)^2\)
  \item Expand and simplify: \((x + 4)(x - 4)\)
  \item Expand and simplify: \((2x + 3)^2\)
  \item Simplify: \((5x - 1)(5x + 1)\)
\end{enumerate}

\subsection*{Part E: Applications and Multi-Term Products}
\begin{enumerate}
  \setcounter{enumi}{20}
  \item Find the area of a rectangle with sides \((x + 3)\) and \((x + 5)\).
  \item Expand: \((x + 2)(x^2 + 3x + 1)\)
  \item Expand: \((x^2 + 2x)(x - 3)\)
  \item Expand: \((2x + 1)(x^2 + 4x + 3)\)
  \item A square garden has side length \((x + 6)\). Write an expression for its area.
\end{enumerate}

\newpage

% ============================================================
% SOLUTIONS — UNIT 6, TOPIC 5: ADDING, SUBTRACTING, AND MULTIPLYING POLYNOMIALS
% ============================================================

\section*{Answer Key and Solutions: Adding, Subtracting, and Multiplying Polynomials}

\subsection*{Part A Solutions: Adding and Subtracting Simple Polynomials}
\begin{enumerate}
  \item \((3x^2 + 5x + 2) + (4x^2 + 3x - 7)\)

  Combine like terms:
  \[
  (3x^2 + 4x^2) + (5x + 3x) + (2 - 7)
  = 7x^2 + 8x - 5.
  \]

  \(\boxed{7x^2 + 8x - 5}\)

  \item \((6x^2 - 2x + 9) - (x^2 + 4x - 3)\)

  Distribute the negative:
  \[
  6x^2 - 2x + 9 - x^2 - 4x + 3
  = (6x^2 - x^2) + (-2x - 4x) + (9 + 3)
  = 5x^2 - 6x + 12.
  \]

  \(\boxed{5x^2 - 6x + 12}\)

  \item \((5x^3 - 2x + 1) + (3x^3 + x - 4)\)

  \[
  (5x^3 + 3x^3) + (-2x + x) + (1 - 4)
  = 8x^3 - x - 3.
  \]

  \(\boxed{8x^3 - x - 3}\)

  \item \((2x^4 + 7x^2 - 3) - (x^4 - 2x^2 + 6)\)

  \[
  2x^4 + 7x^2 - 3 - x^4 + 2x^2 - 6
  = (2x^4 - x^4) + (7x^2 + 2x^2) + (-3 - 6)
  = x^4 + 9x^2 - 9.
  \]

  \(\boxed{x^4 + 9x^2 - 9}\)

  \item \((4x^3 + 2x^2 - 5x) - (6x^3 - 3x^2 + x)\)

  \[
  4x^3 + 2x^2 - 5x - 6x^3 + 3x^2 - x
  = (4x^3 - 6x^3) + (2x^2 + 3x^2) + (-5x - x)
  = -2x^3 + 5x^2 - 6x.
  \]

  \(\boxed{-2x^3 + 5x^2 - 6x}\)
\end{enumerate}

\subsection*{Part B Solutions: Combining Like Terms and Simplifying Expressions}
\begin{enumerate}
  \setcounter{enumi}{5}
  \item \(3x^2 + 2x - 5 + 7x^2 - 4x + 9\)

  \[
  (3x^2 + 7x^2) + (2x - 4x) + (-5 + 9)
  = 10x^2 - 2x + 4.
  \]

  \(\boxed{10x^2 - 2x + 4}\)

  \item \(2x^3 - 4x + 6 - (x^3 + 5x - 2)\)

  \[
  2x^3 - 4x + 6 - x^3 - 5x + 2
  = (2x^3 - x^3) + (-4x - 5x) + (6 + 2)
  = x^3 - 9x + 8.
  \]

  \(\boxed{x^3 - 9x + 8}\)

  \item \(5x^4 + 3x^2 - (2x^4 - 7x^2 + 8)\)

  \[
  5x^4 + 3x^2 - 2x^4 + 7x^2 - 8
  = (5x^4 - 2x^4) + (3x^2 + 7x^2) - 8
  = 3x^4 + 10x^2 - 8.
  \]

  \(\boxed{3x^4 + 10x^2 - 8}\)

  \item \((x^2 + 4x + 1) + (2x^2 - 6x + 9)\)

  \[
  (x^2 + 2x^2) + (4x - 6x) + (1 + 9)
  = 3x^2 - 2x + 10.
  \]

  \(\boxed{3x^2 - 2x + 10}\)

  \item \((x^3 - 5x + 3) - (2x^3 - 4x + 8)\)

  \[
  x^3 - 5x + 3 - 2x^3 + 4x - 8
  = (x^3 - 2x^3) + (-5x + 4x) + (3 - 8)
  = -x^3 - x - 5.
  \]

  \(\boxed{-x^3 - x - 5}\)
\end{enumerate}

\subsection*{Part C Solutions: Multiplying Binomials (FOIL Method)}
\begin{enumerate}
  \setcounter{enumi}{10}
  \item \((x + 3)(x + 7)\)

  \[
  x\cdot x + x \cdot 7 + 3 \cdot x + 3 \cdot 7
  = x^2 + 7x + 3x + 21
  = x^2 + 10x + 21.
  \]

  \(\boxed{x^2 + 10x + 21}\)

  \item \((x - 2)(x + 5)\)

  \[
  x \cdot x + x \cdot 5 - 2 \cdot x - 2 \cdot 5
  = x^2 + 5x - 2x - 10
  = x^2 + 3x - 10.
  \]

  \(\boxed{x^2 + 3x - 10}\)

  \item \((2x + 4)(x + 1)\)

  \[
  2x \cdot x + 2x \cdot 1 + 4 \cdot x + 4 \cdot 1
  = 2x^2 + 2x + 4x + 4
  = 2x^2 + 6x + 4.
  \]

  \(\boxed{2x^2 + 6x + 4}\)

  \item \((3x - 2)(x - 5)\)

  \[
  3x \cdot x + 3x \cdot (-5) - 2 \cdot x - 2 \cdot (-5)
  = 3x^2 - 15x - 2x + 10
  = 3x^2 - 17x + 10.
  \]

  \(\boxed{3x^2 - 17x + 10}\)

  \item \((x + 6)^2\)

  \[
  (x + 6)(x + 6)
  = x^2 + 6x + 6x + 36
  = x^2 + 12x + 36.
  \]

  \(\boxed{x^2 + 12x + 36}\)
\end{enumerate}

\subsection*{Part D Solutions: Recognizing Special Products}
\begin{enumerate}
  \setcounter{enumi}{15}
  \item \((a + b)^2\)

  Pattern: \(a^2 + 2ab + b^2.\)

  \(\boxed{a^2 + 2ab + b^2}\)

  \item \((a - b)^2\)

  Pattern: \(a^2 - 2ab + b^2.\)

  \(\boxed{a^2 - 2ab + b^2}\)

  \item \((x + 4)(x - 4)\)

  Difference of squares:
  \[
  x^2 - 16.
  \]

  \(\boxed{x^2 - 16}\)

  \item \((2x + 3)^2\)

  \[
  (2x + 3)(2x + 3)
  = 4x^2 + 6x + 6x + 9
  = 4x^2 + 12x + 9.
  \]

  \(\boxed{4x^2 + 12x + 9}\)

  \item \((5x - 1)(5x + 1)\)

  Difference of squares:
  \[
  (5x)^2 - 1^2 = 25x^2 - 1.
  \]

  \(\boxed{25x^2 - 1}\)
\end{enumerate}

\subsection*{Part E Solutions: Applications and Multi-Term Products}
\begin{enumerate}
  \setcounter{enumi}{20}
  \item Rectangle with sides \((x + 3)\) and \((x + 5)\)

  Area:
  \[
  (x + 3)(x + 5)
  = x^2 + 5x + 3x + 15
  = x^2 + 8x + 15.
  \]

  \(\boxed{x^2 + 8x + 15}\)

  \item \((x + 2)(x^2 + 3x + 1)\)

  Distribute \(x + 2\):
  \[
  x(x^2 + 3x + 1) + 2(x^2 + 3x + 1)
  = (x^3 + 3x^2 + x) + (2x^2 + 6x + 2)
  = x^3 + 5x^2 + 7x + 2.
  \]

  \(\boxed{x^3 + 5x^2 + 7x + 2}\)

  \item \((x^2 + 2x)(x - 3)\)

  Distribute:
  \[
  x^2(x - 3) + 2x(x - 3)
  = (x^3 - 3x^2) + (2x^2 - 6x)
  = x^3 - x^2 - 6x.
  \]

  \(\boxed{x^3 - x^2 - 6x}\)

  \item \((2x + 1)(x^2 + 4x + 3)\)

  Distribute:
  \[
  2x(x^2 + 4x + 3) + 1(x^2 + 4x + 3)
  = (2x^3 + 8x^2 + 6x) + (x^2 + 4x + 3)
  = 2x^3 + 9x^2 + 10x + 3.
  \]

  \(\boxed{2x^3 + 9x^2 + 10x + 3}\)

  \item Square garden with side \((x + 6)\)

  Area:
  \[
  (x + 6)^2 = x^2 + 12x + 36.
  \]

  \(\boxed{x^2 + 12x + 36}\)
\end{enumerate}

\end{document}
